Proof progress

impl/kafka.v
@@ -70,7 +70,7 @@ Inductive Subtype : list (id * id) -> ct -> type -> type -> Prop :=
 with Md_Subtypes : list (id * id) -> ct -> list md -> list md -> Prop :=
      | MDCons : forall m x x' t1 t1' t2 t2' e e' mu k r mds,
          (In (Method m x' t1' t2' e') mds) ->
-         (Subtype mu k t1' t1) -> (Subtype mu k t2 t2') -> (Md_Subtypes mu k mds r) -> 
+         (Subtype mu k t1 t1') -> (Subtype mu k t2' t2) -> (Md_Subtypes mu k mds r) -> 
          (Md_Subtypes mu k mds ((Method m x t1 t2 e)::r))
      | MDNil : forall mu k mds, (Md_Subtypes mu k mds nil).
 Scheme subtyping_ind := Induction for Subtype Sort Prop
@@ -125,7 +125,8 @@ with HasTypeExpr : env -> heap -> ct -> expr -> type -> Prop :=
     In (a,(HCell(C,a'))) s ->
     Subtype nil k (class C) t ->
     HasTypeExpr g s k (Ref a) t
-| KTREFANY : forall g s k a,
+| KTREFANY : forall g s k a hc,
+    In (a,hc) s -> 
     HasTypeExpr g s k (Ref a) Any
 with HasTypes : env -> heap -> ct -> list expr -> list fd -> Prop :=
      | HTSCONS : forall g s k e t f er fr,
@@ -165,6 +166,7 @@ Proof.
   - intros. eapply KTREFREAD; eauto. apply in_app_iff. eauto.
   - intros. eapply KTREFWRITE; eauto. apply in_app_iff. eauto.
   - intros. eapply KTREFTYPE; eauto. apply in_app_iff. eauto.
+  - intros. eapply KTREFANY; eauto. apply in_app_iff. eauto.
 Qed.
 
 Lemma mu_weakening : forall mu mu' k t1 t2,
@@ -178,7 +180,12 @@ Qed.
 
 Lemma subtype_transitive : forall mu k t1 t2 t3,
   Subtype mu k t1 t2 -> Subtype mu k t2 t3 -> Subtype mu k t1 t3. 
-Admitted. 
+Admitted.
+
+Lemma subtype_method_containment : forall k C D md,
+    Subtype nil k (class C) (class D) -> In md (methods D k) ->
+    exists md', In md' (methods C k) /\ Md_Subtypes nil k (md'::nil) (md::nil).
+Admitted.
 
 (* [thisref/this][varref/var](exp) *)
 Fixpoint subst(thisref : ref)(varref : ref)(var : id)(exp : expr) :=
@@ -254,7 +261,7 @@ Proof.
         ** apply eventually_concrete in H2. inversion H2 as [t' (H5, H6)].
            inversion H6; subst. 
            **** eapply KTREFTYPE with (C:=C0); eauto. apply subtype_transitive with (t2 := t'); eauto.
-           **** inversion H5. subst. apply KTREFANY. 
+           **** inversion H5. subst. eapply KTREFANY; eauto.
         ** apply Nat.eqb_neq in Hxx. inversion H3; 
            assert (Heq : x0 = x0) by reflexivity; contradiction.
       * inversion H4.
@@ -277,10 +284,14 @@ Inductive WellFormedField : ct -> fd -> Prop :=
 | WFFWF : forall f k t, WellFormedType k t -> WellFormedField k (Field f t).
 
 Inductive WellFormedMethod : env -> heap -> ct -> md -> Prop :=
-| WFMDUT : forall x g s k e m, HasType ((x,Any)::g) s k e Any -> WellFormedMethod g s k (Method m x Any Any e)
-| WFMT : forall g s k C1 C2 x e m, WellFormedType k (class C1) -> WellFormedType k (class C2) ->
-         HasType ((x,(class C1)) :: g) s k e (class C2) ->
-         WellFormedMethod g s k (Method m x (class C1) (class C2) e).
+| WFMDUT : forall x g s k e m, x <> this ->
+                               HasType (g ++ (x,Any)::nil) s k e Any ->
+                               WellFormedMethod g s k (Method m x Any Any e)
+| WFMT : forall g s k C1 C2 x e m,
+    x <> this ->
+    WellFormedType k (class C1) -> WellFormedType k (class C2) ->
+    HasType (g ++ (x,(class C1))::nil) s k e (class C2) ->
+    WellFormedMethod g s k (Method m x (class C1) (class C2) e).
 
 Inductive NoDupsMds : list md -> Prop :=
 | NDUPTC : forall m x C D e mds,
@@ -296,6 +307,10 @@ Inductive NoDupsMds : list md -> Prop :=
 Inductive NoDupsFds : list fd -> Prop :=
 | NDUPFD : forall f t fds, NoDupsFds fds -> (forall t', ~ (In (Field f t') fds)) -> NoDupsFds ((Field f t)::fds).
 
+Inductive NoDupsClasses : list k -> Prop :=
+| NDUPK : forall C fds mds ks, NoDupsClasses ks -> (forall fds' mds', ~(In (ClassDef C fds' mds') ks)) ->
+          NoDupsClasses ((ClassDef C fds mds)::ks).
+
 Inductive WellFormedClass : heap -> ct -> k -> Prop :=
 | WFWC : forall s k C mds fds,
     (forall fd, In fd fds -> WellFormedField k fd) ->
@@ -303,13 +318,11 @@ Inductive WellFormedClass : heap -> ct -> k -> Prop :=
     NoDupsFds fds -> NoDupsMds mds -> 
     WellFormedClass s k (ClassDef C fds mds).
 
-Inductive WellFormedClassTable : heap -> ct -> ct -> Prop :=
-| WFCTC : forall c C fds mds s k kr, 
-    c = ClassDef C fds mds -> 
-    (forall fd' md', ~In (ClassDef C fd' md') kr) ->
-    (WellFormedClass s k c) -> WellFormedClassTable s k kr ->
-    WellFormedClassTable s k (c::kr)
-| WFNIL : forall s k, WellFormedClassTable s k nil.
+Inductive WellFormedClassTable : heap -> ct -> Prop :=
+| WFCT : forall s k,
+    (forall C fds mds, In (ClassDef C fds mds) k -> WellFormedClass s k (ClassDef C fds mds)) ->
+    NoDupsClasses k ->
+    WellFormedClassTable s k.
 
 Inductive FieldRefWellFormed : ct -> heap -> list fd -> list ref -> Prop :=
 | FRWF_Cons : forall k s f t fds a a', HasType nil s k (Ref a) t ->
@@ -328,7 +341,7 @@ Inductive WellFormedHeap : ct -> heap -> Prop :=
 
 Inductive WellFormedState : ct -> expr -> heap -> Prop :=
 | WFSWP : forall k e s t, HasType nil s k e t -> WellFormedHeap k s ->
-          WellFormedClassTable s k k ->
+          WellFormedClassTable s k ->
           WellFormedState k e s.
 
 (* all exprs are refs in a list *)
@@ -362,37 +375,37 @@ Proof.
   - eapply WFWTC. apply H.
 Qed.
 
-Lemma fields_gets_fields : forall C s k k' fds, 
-    WellFormedType k (class C) -> WellFormedClassTable s k' k ->
+Lemma fields_gets_fields : forall C s k fds, 
+    WellFormedType k (class C) -> WellFormedClassTable s k ->
     fields C k = fds <-> exists mds, In (ClassDef C fds mds) k.
 Proof.
-  intros C s k k' fds H H0. split; intros H1. 
+  intros C s k fds H H0. destruct H0 as [s k _ Hdups]. split; intros H1. 
   - induction k as [n | k''].
-    + inversion H. subst. inversion H4.
+    + inversion H. subst. inversion H3.
     + destruct k'' as [C' fds' mds']. simpl in H1. destruct (Nat.eqb C C') eqn:HCC.
       * apply Nat.eqb_eq in HCC. subst. exists mds'. simpl. auto. 
       * apply Nat.eqb_neq in HCC. simpl. inversion H. subst. apply strong_weakening_of_type_wf in H; eauto. 
         apply IHk in H; eauto.
         ** inversion H as [mds'' H5]. exists mds''. auto.
-        ** inversion H0. subst. eauto. 
+        ** inversion Hdups. apply H2. 
   - induction k as [|k''].
-    + inversion H1. inversion H2. 
+    + inversion H1. inversion H0. 
     + destruct k'' as [C' fds' mds']. unfold fields. destruct (C =? C') eqn:HCC.
       * apply Nat.eqb_eq in HCC. subst. inversion H1. inversion H0.
         ** subst. inversion H2.
-           *** inversion H3. subst. reflexivity. 
-           *** inversion H5. subst. unfold not in H6. apply H6 in H3. contradiction.
+           *** inversion H2. subst. reflexivity.
+        ** inversion Hdups. subst. apply H8 in H2. tauto.
       * apply IHk.
         ** eapply strong_weakening_of_type_wf; eauto. apply Nat.eqb_neq in HCC. apply HCC.
-        ** inversion H0. eauto.
-        ** inversion H1. inversion H2.
-           *** inversion H3. apply Nat.eqb_neq in HCC. symmetry in H5. contradiction.
+        ** inversion Hdups. tauto. 
+        ** inversion H1. inversion H0.
+           *** inversion H2. apply Nat.eqb_neq in HCC. symmetry in H5. subst. contradiction.
            *** exists x. eauto. 
 Qed.
 
 Lemma heap_wf_field_access : forall k s a C aps f t a',
     WellFormedHeap k s ->
-    WellFormedClassTable s k k ->
+    WellFormedClassTable s k ->
     In (a, HCell(C, aps)) s -> FieldIn f t a' (fields C k) aps ->
   HasType nil s k (Ref a') t.
 Proof.
@@ -418,24 +431,13 @@ Inductive FieldWrite : id -> ref -> list ref -> list fd -> list ref -> Prop :=
     f <> f' -> FieldWrite f a aps fs aps' -> FieldWrite f a (a'::aps) ((Field f' t)::fs) (a' :: aps').
 
 Lemma FieldsNoDupsFds : forall s (k k' : ct) (C : id) fds mds, 
-    WellFormedClassTable s k' k ->
+    WellFormedClassTable s k ->
     In (ClassDef C fds mds) k ->
     fds = (fields C k) ->
     NoDupsFds fds.
 Proof.
-  intros s k k' C fds mds H H0 H1. induction k.
-  - inversion H0.
-  - inversion H0.
-    + inversion H. subst fds. subst.
-      inversion H9. subst.  
-      inversion H2.  rewrite <- H4. unfold fields.
-      rewrite Nat.eqb_refl. apply H12.
-    + apply IHk; eauto.
-      * inversion H. subst. apply H10.
-      * clear H1. clear IHk. clear H0. symmetry. rewrite fields_gets_fields with (s := s) (k' := k').
-        ** exists mds. apply H2. 
-        ** eapply WFWTC.  apply H2.
-        ** inversion H. apply H8. 
+  intros s k k' C fds mds H H0 H1. inversion H.
+  apply H2 in H0. inversion H0. subst. apply H13.
 Qed.
 
 Lemma FieldWriteWellFormed : forall (k k' : ct) s a fds ais ais' t f,
@@ -462,24 +464,16 @@ Proof.
 Qed.
 
 Lemma no_two_classes : forall s k C fds mds fds' mds',
-    WellFormedClassTable s k k -> In (ClassDef C fds mds) k -> In (ClassDef C fds' mds') k ->
+    WellFormedClassTable s k -> In (ClassDef C fds mds) k -> In (ClassDef C fds' mds') k ->
     fds = fds' /\ mds = mds'.
 Proof.
-  intros. induction H.
-  - subst. destruct (Nat.eqb C C0) eqn:HCC.
-    + apply Nat.eqb_eq in HCC. subst. inversion H0.
-      * inversion H. subst. inversion H1.
-        ** inversion H5. auto.
-        ** apply H2 in H5. contradiction. 
-      * apply H2 in H. contradiction.
-    + apply Nat.eqb_neq in HCC. inversion H0.
-      * inversion H. subst. tauto.
-      * apply IHWellFormedClassTable in H.
-        ** apply H.
-        ** inversion H1.
-           *** inversion H5. subst. tauto. 
-           *** apply H5.
-  - inversion H0. 
+  intros. inversion H. subst. clear H2. clear H. induction k0.
+  - inversion H0.
+  - inversion H0; inversion H1.
+    + subst. inversion H2. eauto.
+    + subst. inversion H3. subst. apply H8 in H2. tauto.
+    + inversion H3. subst. inversion H4. subst. apply H7 in H. tauto.
+    + apply IHk0; eauto. inversion H3. apply H6.
 Qed.
 
 Lemma heap_write_still_in : forall a s s' a' aps' hc,
@@ -528,6 +522,7 @@ Proof.
     + apply in_or_app. eauto.
   - intros. apply KTREFTYPE with (a' := a') (C := C); eauto.
     apply in_or_app. eauto.
+  - intros. eapply KTREFANY. apply in_or_app. eauto.
 Qed.
 
 Lemma subtype_only_classes : forall mu k C t, Subtype mu k (class C) t -> exists D, t = (class D).
@@ -537,49 +532,69 @@ Proof.
   - subst. exists t2. reflexivity.
   - subst. exists d. reflexivity.
 Qed.
-   
-Lemma hastype_ignores_heapv : forall (k:ct) (s s':heap) a a' aps' t,
-    WellFormedHeap k s ->
-    HasType nil s k (Ref a) t ->
-    HeapWrite a' aps' s s' -> 
-    HasType nil s' k (Ref a) t.
+
+
+Require Import Coq.Program.Tactics.
+Definition retains_references(s1:heap)(s2:heap) :=
+  forall a C aps, In (a, HCell(C,aps)) s1 -> exists aps', In(a, HCell(C,aps')) s2.
+
+Lemma heapwrite_retains_refs' : forall a aps' s s',
+    HeapWrite a aps' s s' -> retains_references s s'.
 Proof.
-  intros.
-  assert (Hduh: s' = s').
-  { reflexivity. }
-  assert (Hduh2: (Ref a) = (Ref a)).
-  { reflexivity. }
-  generalize dependent Hduh. generalize dependent Hduh2.
-   (* pose proof typing_ind (fun g s k e t (ih : HasType g s k e t) => e = (Ref a) -> s = s' -> HasType nil s' k (Ref a) t). eapply H2. *)
-  eapply typing_ind with (P := fun g s k e t (ih : HasType g s k e t) => e = (Ref a) -> s = s' -> HasType nil s' k (Ref a) t)
-                           (P0 := fun g s k e t ih => e = (Ref a) -> s = s' -> HasTypeExpr nil s' k (Ref a) t)
-                           (P1 := fun g s k es ts ih => True) (e:= nil); try (intros; subst; discriminate); eauto.
-  - intros. subst. inversion H2. subst. eauto.
-  - apply eventually_concrete in H0. destruct H0 as [tp [H2 H3]]. inversion H3.
-    + subst. inversion H. subst. clear H H5. induction H1.
-      * destruct (Nat.eqb a0 a) eqn:Heq.
-        ** apply Nat.eqb_eq in Heq. subst. inversion H4.
-           *** inversion H. subst. apply KTEXPR. eapply KTREFTYPE; eauto.
-               **** apply in_eq.
-               **** pose proof subtype_transitive (nil) k0 (class C) tp t H8 H2. apply H1. 
-           *** inversion H0. apply H6 in H. tauto.
-        ** apply Nat.eqb_neq in Heq. inversion H4.
-           *** inversion H. subst. tauto.
-           *** apply KTEXPR. eapply KTREFTYPE; eauto.
-               **** apply in_cons. apply H.
-               **** eapply subtype_transitive; eauto. 
-      * destruct (Nat.eqb a' a) eqn:Heq.
-        ** apply Nat.eqb_eq in Heq. subst. inversion H4.
-           *** inversion H5. subst. apply KTEXPR. apply KTREFTYPE with (C:=C) (a' := a'0). 
-               **** apply in_eq.
-               **** eapply subtype_transitive; eauto.
-           *** inversion H0. apply H9 in H5. tauto.
-        ** apply Nat.eqb_neq in Heq. inversion H4.
-           *** inversion H5. subst. tauto.
-           *** apply heap_weakening_2 with (s' := (a',HCell(C0,aps')) :: nil). apply IHHeapWrite; eauto.
-               **** apply nodupsheap_weakening in H0. apply H0.
-    + subst. inversion H2. subst. apply KTEXPR. apply KTREFANY.
+  intros. induction H.
+  - unfold retains_references. intros. destruct (Nat.eq_dec C0 C); destruct (Nat.eq_dec a0 a).
+    + subst. exists aps. apply in_eq.
+    + subst. inversion H.
+      * exists aps. inject H0. tauto.
+      * exists aps0. apply in_cons. tauto.
+    + subst. inversion H.
+      * inject H0. exists aps. tauto.
+      * exists aps0. apply in_cons. tauto.
+    + inversion H.
+      * inject H0. tauto.
+      * exists aps0. apply in_cons. tauto.
+  - unfold retains_references. intros. inversion H1.
+    + inject H2. exists aps0. apply in_eq.
+    + unfold retains_references in IHHeapWrite.
+      apply IHHeapWrite in H2. destruct H2. exists x. apply in_cons. apply H2. 
 Qed.
+
+Lemma retain_references_ref : forall s, retains_references s s.
+Proof.
+  intros. unfold retains_references; intros. exists aps. apply H.
+Qed.
+Hint Resolve retain_references_ref.
+
+
+Lemma hastype_ignores_heapv'' : forall s s' k g e t,
+    HasType g s k e t -> retains_references s s' -> HasType g s' k e t.
+Proof.
+  intros. 
+  pose proof (eq_refl k0) as Hduh1.
+  pose proof (eq_refl s) as Hduh2.
+  generalize dependent Hduh1. generalize dependent Hduh2.
+  apply typing_ind with
+  (P:= fun g s'' k' e t ih => s'' = s -> k' = k0 -> HasType g s' k0 e t)
+    (P0 := fun g s'' k' e t ih => s'' = s -> k' = k0 -> HasTypeExpr g s' k0 e t)
+    (P1 := fun g s'' k' es ts ih => s'' = s -> k' = k0 -> HasTypes g s' k0 es ts);
+    try (intros; subst; eauto; fail). 
+  - intros. subst. unfold retains_references in H0. apply H0 in i. destruct i as [aps' H1]. eapply KTREFREAD; eauto.
+  - intros. subst. unfold retains_references in H0. apply H0 in i. destruct i as [aps' H2]. eauto.
+  - intros. subst. unfold retains_references in H0. apply H0 in i. destruct i as [aps' H1]. eauto.
+  - intros. subst. unfold retains_references in H0. destruct hc.  destruct p.
+    apply H0 in i. destruct i as [aps' H1]. eauto.
+Qed.
+Hint Resolve hastype_ignores_heapv''.
+
+   
+Lemma hastype_ignores_heapv : forall (k:ct) (s s':heap) g a a' aps' t,
+    HasType g s k (Ref a) t ->
+    HeapWrite a' aps' s s' -> 
+    HasType g s' k (Ref a) t.
+Proof.
+  intros. eapply hastype_ignores_heapv''.  eauto. eapply heapwrite_retains_refs'; eauto.
+Qed.
+Hint Resolve hastype_ignores_heapv.
 
 Lemma fieldwf_still_good : forall k s a' s' fds aps' aps, 
   WellFormedHeap k s ->
@@ -596,15 +611,15 @@ Proof.
   - apply FRWF_Nil.
 Qed.
 
-Lemma writing_keeps_refs : forall a a' s s' aps' hc,
-    In(a,hc) s -> HeapWrite a' aps' s s' -> exists hc', In(a,hc') s'.
+Lemma writing_keeps_refs : forall a a' s s' aps' C aps,
+    In(a,HCell(C,aps)) s -> HeapWrite a' aps' s s' -> exists aps', In(a,HCell(C, aps')) s'.
 Proof.
   intros. induction H0.
   - inversion H.
-    + inversion H0. subst.  exists (HCell(C,aps)). apply in_eq.
-    + exists hc. apply in_cons. apply H0.
+    + inversion H0. subst. exists aps0. apply in_eq.
+    + exists aps. apply in_cons. apply H0.
   - inversion H.
-    + inversion H2. subst. exists (HCell(C,aps')). apply in_eq.
+    + inversion H2. subst. exists aps. apply in_eq.
     + apply IHHeapWrite in H2. inversion H2 as [hc' H3]. exists hc'.
       apply in_cons. apply H3.
 Qed.
@@ -724,7 +739,7 @@ Qed.
 
 Lemma write_field : forall s s' k a a' aps aps' t C f,
     WellFormedHeap k s ->
-    WellFormedClassTable s k k ->
+    WellFormedClassTable s k ->
     HasType nil s k (Ref a) t ->
     In (Field f t) (fields C k) ->
     In (a', HCell(C, aps)) s ->
@@ -737,7 +752,7 @@ Proof.
 
   inversion Hwfh.
   subst. pose proof Hobj. apply H0 in H1. destruct H1. remember (fields C k) as fds.
-  pose proof (fields_gets_fields C s k k fds H1 Hwfct). symmetry in Heqfds. pose proof Heqfds.
+  pose proof (fields_gets_fields C s k fds H1 Hwfct). symmetry in Heqfds. pose proof Heqfds.
   apply H3 in Heqfds.
   destruct Heqfds as [mds H5]. 
     
@@ -784,10 +799,12 @@ Inductive Steps : ct -> expr -> heap -> ct -> expr -> heap -> Prop :=
     FieldWrite f a' aps (fields C k) aps' ->
     HeapWrite a aps' s s' ->
     Steps k (SetF (Ref a) f (Ref a')) s k (Ref a') s'
-| SCall : forall a C aps s m x t t' e k a',
+| SCall : forall a C aps s m x t1 t1' t2 t2' e k a',
     In (a, HCell(C,aps)) s ->
-    In (Method m x t t' e) (methods C k) ->
-    Steps k (Call (Ref a) m t t' (Ref a')) s k (subst a a' x e) s
+    In (Method m x t1 t2 e) (methods C k) ->
+    Subtype nil k t1' t1 ->
+    Subtype nil k t2 t2' ->
+    Steps k (Call (Ref a) m t1' t2' (Ref a')) s k (subst a a' x e) s
 | SDynCast : forall k a s, Steps k (SubCast Any (Ref a)) s k (Ref a) s
 | SSubCast : forall a aps C D s k,
     In (a, HCell(C,aps)) s ->
@@ -795,4 +812,390 @@ Inductive Steps : ct -> expr -> heap -> ct -> expr -> heap -> Prop :=
     Steps k (SubCast (class D) (Ref a)) s k (Ref a) s
 | SCtx : forall k e s e' s' E,
     Steps k e s k e' s' -> Steps k (equivExpr e E) s k (equivExpr e' E) s'.
-    
+Hint Constructors Steps.
+Hint Constructors EvalCtx.
+
+Fixpoint typesof(fds : list fd) : list type :=
+  match fds with
+    (Field f t) :: r => t :: (typesof r)
+  | nil => nil
+  end.
+
+Hint Constructors WellFormedState.
+
+
+Lemma infields_implies_fieldin : forall k f s t a C aps,
+    WellFormedHeap k s ->
+    WellFormedClassTable s k ->
+    In (a, HCell(C,aps)) s -> 
+    In (Field f t) (fields C k) -> exists a', FieldIn f t a' (fields C k) aps.
+Proof.
+  intros. destruct H. apply H3 in H1. clear H3. destruct H1. remember (fields C k0) as fds.
+  pose proof (fields_gets_fields C s k0 fds H1 H0). destruct H4. clear H5. symmetry in Heqfds.
+  pose proof Heqfds as Heqfds'. apply H4 in Heqfds. destruct Heqfds as [mds Hin]. clear H4. symmetry in Heqfds'.
+  pose proof (FieldsNoDupsFds s k0 k0 C fds mds H0 Hin Heqfds').
+  clear Heqfds'. clear Hin H0 H1. clear mds H.
+  induction H3.
+  - destruct (Nat.eq_dec f f0); subst.
+    + inject H2.
+      * inject H0. exists a0. apply FieldIn_Here.
+      * inject H4. apply H7 in H0. tauto.
+    + inject H2.
+      * inject H0. tauto.
+      * inject H4. destruct (IHFieldRefWellFormed H0 H5) as [a0' H8].
+        exists a0'. apply FieldIn_Next; eauto.
+  - inversion H2.
+Qed.
+
+Fixpoint update_field_ref(f:id)(a:ref)(fds:list fd)(aps:list ref) : list ref :=
+  match fds, aps with
+    (Field f' t)::fr, a'::ar => match Nat.eqb f f' with
+                                    true => a :: ar
+                                  | false => a' :: (update_field_ref f a fr ar)
+                                  end
+  | _, _ => nil
+  end.
+
+Lemma update_field_is_well_formed : forall f t a k s aps aps' fds,
+    FieldRefWellFormed k s fds aps ->
+    (In (Field f t) fds) ->
+    update_field_ref f a fds aps = aps' ->
+    FieldWrite f a aps fds aps'.
+Proof.
+  intros. subst. induction H.
+  - unfold update_field_ref. destruct (f =? f0) eqn:Hff.
+    + apply Nat.eqb_eq in Hff. subst. apply FWC.
+    + apply FWN.
+      * apply Nat.eqb_neq. eauto.
+      * apply IHFieldRefWellFormed; eauto. inversion H0; eauto. inject H2. apply Nat.eqb_neq in Hff.
+        tauto.
+  - inversion H0.
+Qed.
+
+Fixpoint update_heap(a:ref)(aps:list ref)(s:heap) : heap :=
+  match s with
+  | (a',HCell(C,aps'))::ar => match Nat.eqb a a' with
+                                true => (a,HCell(C,aps))::ar
+                              | false => (a',HCell(C,aps'))::(update_heap a aps ar)
+                              end
+  | nil => nil
+  end.
+Lemma update_heap_writes : forall s a C aps aps',
+  (In (a,HCell(C, aps')) s) ->
+  HeapWrite a aps s (update_heap a aps s).
+Proof.
+  intros. induction s.
+  - inversion H.
+  - unfold update_heap. destruct a0 as [a' [(C', aps'')]]. destruct (a =? a') eqn:Heq.
+    + apply Nat.eqb_eq in Heq. subst. apply HWC.
+    + apply Nat.eqb_neq in Heq. apply HWNC; eauto. apply IHs. inject H; eauto. inject H0. tauto.
+Qed.
+
+Lemma hastype_ignores_heapv' : forall (k : ct) (s s' : heap) (g : env)
+                                      (a' : id) (aps' : list ref) (t : type) e,
+    HasType g s k e t ->
+    HeapWrite a' aps' s s' -> HasType g s' k e t.
+Proof.
+  intros. eapply hastype_ignores_heapv''. eauto. eapply heapwrite_retains_refs'. eauto.
+Qed.
+
+Lemma wfm_doesnt_care : forall md g s k s',
+    WellFormedMethod g s k md ->
+    retains_references s s' ->
+    WellFormedMethod g s' k md.
+Proof.
+  intros. inject H.
+  - apply WFMDUT; eauto. 
+  - apply WFMT; eauto. 
+Qed.
+
+Lemma wfc_doesnt_care : forall s k c s',
+  WellFormedClass s k c ->
+  retains_references s s' ->
+  WellFormedClass s' k c.
+Proof.
+  intros. inject H. eapply WFWC; eauto. intros. remember ((this, class C) :: nil) as g.
+  apply H2 in H. eapply wfm_doesnt_care in H; eauto.
+Qed.
+
+Lemma wfct_doesnt_care : forall s s' k, 
+  WellFormedClassTable s k ->
+  retains_references s s' ->
+  WellFormedClassTable s' k.
+Proof.
+  intros. inject H. apply WFCT.
+  - intros. eapply wfc_doesnt_care; eauto.
+  - eauto. 
+Qed.
+
+
+Lemma methods_in : forall fds mds s C k,
+    WellFormedClassTable s k ->
+    In (ClassDef C fds mds) k ->
+    mds = (methods C k).
+Proof.
+  intros. destruct H as [s k _ H]. induction k.
+  - inversion H0.
+  - destruct a as [D fds' mds']. destruct (Nat.eq_dec C D).
+    + subst. simpl. rewrite Nat.eqb_refl. inversion H0; eauto.
+      * inject H1. reflexivity.
+      * inject H. apply H7 in H1. tauto. 
+    + unfold methods. apply Nat.eqb_neq in n. rewrite -> n. apply IHk.
+      * inject H. apply H3.
+      * inversion H0.
+        ** inject H1. apply Nat.eqb_neq in n. tauto.
+        ** apply H1.
+Qed.
+        
+Lemma methods_are_wf : forall s k C mds,
+    WellFormedClassTable s k ->
+    WellFormedType k (class C) ->
+  mds = (methods C k) ->
+  (forall md, In md mds -> WellFormedMethod ((this, class C) :: nil) s k md).
+Proof.
+  intros. inversion H0. subst.
+  pose proof (methods_in fds mds0 s C k0 H H5). rewrite <- H1 in H2. 
+  inversion H. subst. 
+  apply H3 in H5. clear H3 H4. inversion H5.
+  subst. apply H9 in H2. eauto.  
+Qed.
+
+Lemma subtype_only_classes' : forall mu k t C,
+    Subtype mu k t (class C) -> exists D, t = (class D).
+Proof.
+  intros. inversion H.
+  - subst. exists C. reflexivity.
+  - subst. exists t1. reflexivity.
+  - eauto.
+Qed.
+
+Definition is_sound(k:ct)(s:heap)(e:expr)(t:type) :=
+  (exists a : ref, e = Ref a) \/
+  (exists (e' : expr) (s' : heap), Steps k e s k e' s' /\
+                                           WellFormedState k e' s' /\
+                                           HasType nil s' k e' t /\
+                                           retains_references s s') \/
+  (exists E : EvalCtx,
+      (exists (a : ref) (m : id) (a' : ref),
+          e = equivExpr (DynCall (Ref a) m (Ref a')) E) \/
+      (exists (t' : type) (a : ref),
+          e = equivExpr (SubCast t' (Ref a)) E)).
+
+
+Theorem soundness: forall k e s t,
+  WellFormedState k e s -> HasType nil s k e t -> is_sound k s e t.
+Proof.
+  intros k e s t Hwfs Hht. destruct Hwfs as [k e s _ _ Hwfh Hwfct].
+  pose proof (eq_refl (@nil (id*type))) as Hduh0.
+  pose proof (eq_refl k) as Hduh1. pose proof (eq_refl s) as Hduh2.    
+  generalize dependent Hduh2. generalize dependent Hduh1. generalize dependent Hduh0.
+  apply typing_ind with
+  (P := fun g' s' k' e t ih =>
+          g' = nil -> k' = k -> s' = s -> is_sound k s e t)
+  (P0 := fun g' s' k' e t ih =>
+           g' = nil -> k' = k -> s' = s -> is_sound k s e t)
+  (P1 := fun g' s' k' es ts (ih : HasTypes g' s' k' es ts) => (* TODO: state IH for list of exprs *)
+           g' = nil -> k' = k -> s' = s -> @Forall2 expr type (is_sound k s) es (typesof ts));
+    try (intros; subst; inversion i; fail); try (intros; subst; unfold is_sound; eauto; fail). 
+  - intros. subst. destruct H; eauto.
+    + unfold is_sound. eauto.
+    + unfold is_sound. right. destruct H.
+      * left. destruct H  as [e' [s' [H1 [H2 [H3 H4]]]]]. exists e'. exists s'. repeat split; eauto.
+      * right. eauto.
+  - intros. subst. destruct H; try (unfold is_sound); eauto.
+  - intros. subst. unfold is_sound. right. left.
+    destruct (infields_implies_fieldin _ _ _ _ _ _ _ Hwfh Hwfct i i0) as [a'' H1].
+    exists (Ref a''). exists s. repeat split; eauto.
+    + eapply WFSWP; eauto. destruct Hwfh. apply a0 in i. destruct i as [_ H2].
+      eapply FieldsWFImpliesFieldIn; eauto.
+    + eapply FieldsWFImpliesFieldIn; eauto. destruct Hwfh. apply H0 in i.
+      destruct i as [_ H2]. eauto. 
+  - intros. subst. destruct H; eauto.
+    * unfold is_sound. right. left. inject H.
+      remember (fields C k) as fds.
+      remember (update_field_ref f x fds a') as aps'.
+      remember (update_heap a aps' s) as s'.
+      exists (Ref x).
+      exists s'. 
+      assert (HHwrite: HeapWrite a aps' s s').
+      { rewrite Heqs'. eapply update_heap_writes; eauto. }
+      assert (HFwrite: FieldWrite f x a' fds aps').
+      { eapply update_field_is_well_formed; eauto. destruct Hwfh. apply a0 in i.
+        inject i. apply H0. }
+      repeat split; try eauto.
+      ** subst. eapply SWrite; eauto.
+      ** eapply WFSWP; eauto.
+         *** eapply write_field.
+             **** apply Hwfh.
+             **** apply Hwfct.
+             **** apply h.
+             **** rewrite Heqfds in i0. apply i0. 
+             **** apply i.
+             **** subst. apply HFwrite. 
+             **** subst. apply HHwrite.
+         *** eapply wfct_doesnt_care; eauto. eapply heapwrite_retains_refs'; eauto.
+      ** eapply heapwrite_retains_refs'; eauto. 
+    * unfold is_sound. right. inject H.
+      ** left. destruct H0 as [e' [s' [HS [Hwfs [Hht' Hret]]]]].
+         remember (EAssign a f (EHole)) as E.
+         assert (Hleft: equivExpr e0 E = SetF (Ref a) f e0).
+         { subst. reflexivity. }
+         assert (Hright: equivExpr e' E = SetF (Ref a) f e').
+         { subst. tauto. }
+         rewrite <- Hleft.  exists (equivExpr e' E). exists s'. apply Hret in i. inversion i.
+         repeat split; try eauto. 
+         *** destruct Hwfs. eapply WFSWP; eauto.
+             **** rewrite -> Hright. eapply KTEXPR. eapply KTREFWRITE; eauto.
+         *** rewrite -> Hright. eapply KTEXPR. eapply KTREFWRITE; eauto.
+      ** right. destruct H0 as [E H1]. remember (EAssign a f E) as E'.
+         exists E'. subst. simpl. inversion H1.
+         *** left. inversion H as [a1 [m1 [a2 H2]]]. exists a1. exists m1. exists a2.
+             rewrite <- H2. reflexivity.
+         *** right. inversion H as [t' [a1 H2]]. exists t'. exists a1. rewrite <- H2. reflexivity.
+  - intros. subst. destruct H; destruct H0; eauto.
+    + destruct H as [a1 H1]. destruct H0 as [a2 H2]. subst. apply eventually_concrete in h.
+      unfold is_sound. right. left.
+      destruct h as [tp [H1 H2]]. inversion H2; eauto.
+      * subst. pose proof (subtype_transitive _ _ _ _ _ H6 H1).
+        apply subtype_method_containment with (md0 := (Method m x t0 t' eb)) in H; eauto.
+        inversion H as [[m' x' t0' t'' e'] [H3 H4]]. inversion H4. subst. inversion H13; eauto.
+        ** inject H5. clear H18.
+           remember (subst a1 a2 x'0 e'0) as ebody. exists ebody. exists s.
+           assert (Hbody: HasType nil s k ebody t2').
+           {
+             pose proof H0 as Hback. inversion Hwfh. subst. apply H7 in H0. destruct H0.
+             pose proof H0. inversion H0. subst. remember (methods C0 k) as mds'.
+             pose proof (methods_are_wf s k C0 mds' Hwfct H9 Heqmds'). subst. apply H10 in H3.
+             inversion H3.
+             **** subst. simpl in H24. eapply substituion_typing; eauto. 
+             **** subst. simpl in H26. eapply substituion_typing; eauto. 
+           }
+           repeat split; eauto.
+           *** rewrite Heqebody. eapply SCall with (C:=C0)(aps := a'); eauto. 
+        ** inversion H5.
+      * subst. inversion H1.
+    + destruct H as [a H]. subst. destruct H0.
+      * unfold is_sound. right. left. inversion H as [e0' [s' [H1 [H2 [H3 H4]]]]].
+        remember (ECall2 a m t0 t' EHole) as E.
+        assert (Hleft: equivExpr e' E = Call (Ref a) m t0 t' e').
+        { subst. tauto. }
+        assert (Hright: equivExpr e0' E = Call (Ref a) m t0 t' e0').
+        { subst. tauto. }
+        assert (Htyped: HasType nil s' k (equivExpr e0' E) t').
+        {
+          rewrite Hright. apply KTEXPR. eapply KTCALL; eauto.
+        }
+         exists (equivExpr e0' E). exists s'.  repeat split; eauto.
+        ** rewrite <- Hleft. eauto.
+        ** eapply WFSWP; eauto.
+           *** inversion H2. apply H5.
+           *** eapply wfct_doesnt_care; eauto.
+      * unfold is_sound. right. right. destruct H as [E H].
+        remember (ECall2 a m t0 t' E) as E'. exists E'. inject H.
+        ** left. inversion H0 as [a' [m' [a'' He]]]. exists a'. exists m'. exists a''.
+           simpl. rewrite He. tauto.
+        ** right. inversion H0 as [t'' [a' He]]. exists t''. exists a'. simpl.
+           rewrite He. tauto.
+    + destruct H.
+      * inversion H as [e0' [s' [H1 [H2 [H3 H4]]]]]. unfold is_sound.
+        right. left.
+        remember (ECall1 EHole m t0 t' e') as E.
+        assert (Hleft: equivExpr e0 E = (Call e0 m t0 t' e')).
+        { subst. tauto. }
+        assert (Hright: equivExpr e0' E = Call e0' m t0 t' e').
+        { subst. tauto. }
+        assert (Htyped: HasType nil s' k (equivExpr e0' E) t').
+        { rewrite Hright. apply KTEXPR. eapply KTCALL; eauto. }
+        exists (equivExpr e0' E). exists s'. repeat split; eauto.
+        ** rewrite<- Hleft. eapply SCtx. apply H1.
+        ** eapply WFSWP; eauto.
+           *** inversion H2. auto.
+           ***  eapply wfct_doesnt_care; eauto.
+      * destruct H as [E H]. remember (ECall1 E m t0 t' e') as E'.
+        unfold is_sound. right. right. exists E'. clear H0. inject H.
+        ** left. inversion H0 as [a' [m' [a'' He]]]. exists a'. exists m'. exists a''.
+           subst. simpl. auto.
+        ** right. inversion H0 as [t'' [a' He]]. exists t''. exists a'. subst. simpl. auto.
+    + destruct H.
+      * inversion H as [e0' [s' [H1 [H2 [H3 H4]]]]]. unfold is_sound.
+        right. left.
+        remember (ECall1 EHole m t0 t' e') as E.
+        assert (Hleft: equivExpr e0 E = (Call e0 m t0 t' e')).
+        { subst. tauto. }
+        assert (Hright: equivExpr e0' E = Call e0' m t0 t' e').
+        { subst. tauto. }
+        assert (Htyped: HasType nil s' k (equivExpr e0' E) t').
+        { rewrite Hright. apply KTEXPR. eapply KTCALL; eauto. }
+        exists (equivExpr e0' E). exists s'. repeat split; eauto.
+        ** rewrite<- Hleft. eapply SCtx. apply H1.
+        ** eapply WFSWP; eauto.
+           *** inversion H2. auto.
+           ***  eapply wfct_doesnt_care; eauto.
+      * destruct H as [E H]. remember (ECall1 E m t0 t' e') as E'.
+        unfold is_sound. right. right. exists E'. clear H0. inject H.
+        ** left. inversion H0 as [a' [m' [a'' He]]]. exists a'. exists m'. exists a''.
+           subst. simpl. auto.
+        ** right. inversion H0 as [t'' [a' He]]. exists t''. exists a'. subst. simpl. auto.
+  - intros. subst. destruct H; destruct H0; eauto.
+    + unfold is_sound. right. right. exists EHole. left.
+      inversion H. inversion H0. exists x. exists m. exists x0. simpl. subst.
+      tauto.
+    + destruct H0.
+      * inversion H0 as [e0' [s' [H1 [H2 [H3 H4]]]]]. unfold is_sound.
+        right. left. inversion H as [a]. subst. remember (EDCall2 a m EHole) as E.
+        assert (Hleft: equivExpr e' E = (DynCall (Ref a) m e')).
+        { subst. tauto. }
+        assert (Hright: equivExpr e0' E = (DynCall (Ref a) m e0')).
+        { subst. tauto. }
+        assert (Htyped: HasType nil s' k (equivExpr e0' E) Any).
+        { subst. simpl. eapply KTEXPR. eapply KTDYNCALL; eauto. }
+        exists (equivExpr e0' E). exists s'. repeat split; eauto.
+        ** rewrite <- Hleft. eapply SCtx; eauto.
+        ** eapply WFSWP; eauto.
+           *** inversion H2; auto.
+           *** eapply wfct_doesnt_care; eauto.
+      * destruct H as [a H]. subst. destruct H0 as [E H0]. remember (EDCall2 a m E) as E'.
+        unfold is_sound. right. right. exists E'. inject H0.
+        ** left. inversion H as [a' [m' [a'' He]]]. exists a'. exists m'. exists a''.
+           subst. eauto.
+        ** right. inversion H as [t'' [a' He]]. exists t''. exists a'. subst. simpl. auto.
+    + destruct H0 as [a H0]. subst. destruct H.
+      * unfold is_sound. right. left. remember (EDCall1 EHole m (Ref a)) as E.
+        inversion H as [e0' [s' [H1 [H2 [H3 H4]]]]].
+        assert (Hleft: equivExpr e0 E = (DynCall e0 m (Ref a))).
+        { subst. tauto. }
+        assert (Hright: equivExpr e0' E = DynCall e0' m (Ref a)).
+        { subst. tauto. }
+        assert (Htyped: HasType nil s' k (equivExpr e0' E) Any).
+        { rewrite Hright. apply KTEXPR. eapply KTDYNCALL; eauto. }
+        exists (equivExpr e0' E). exists s'. repeat split; eauto.
+        ** rewrite <- Hleft. eapply SCtx; eauto.
+        ** eapply WFSWP; eauto.
+           *** inversion H2; auto.
+           *** eapply wfct_doesnt_care; eauto.
+      * unfold is_sound. right. right. destruct H as [E H]. remember (EDCall1 E m (Ref a)) as E'.
+        exists E'. inversion H.
+        ** left. inversion H0 as [a' [m' [a'' He]]]. exists a'. exists m'. exists a''.
+           subst. auto.
+        ** right. inversion H0 as [t'' [a' He]]. exists t''. exists a'. subst. simpl. auto.
+    + clear H0. destruct H.
+      * unfold is_sound. right. left. remember (EDCall1 EHole m e') as E.
+        inversion H as [e0' [s' [H1 [H2 [H3 H4]]]]].
+        assert (Hleft: equivExpr e0 E = (DynCall e0 m e')).
+        { subst. tauto. }
+        assert (Hright: equivExpr e0' E = DynCall e0' m e').
+        { subst. tauto. }
+        assert (Htyped: HasType nil s' k (equivExpr e0' E) Any).
+        { rewrite Hright. apply KTEXPR. eapply KTDYNCALL; eauto. }
+        exists (equivExpr e0' E). exists s'. repeat split; eauto.
+        ** rewrite <- Hleft. eapply SCtx; eauto.
+        ** eapply WFSWP; eauto.
+           *** inversion H2; auto.
+           *** eapply wfct_doesnt_care; eauto.
+      * unfold is_sound. right. right. destruct H as [E H]. remember (EDCall1 E m e') as E'.
+        exists E'. inversion H.
+        ** left. inversion H0 as [a' [m' [a'' He]]]. exists a'. exists m'. exists a''.
+           subst. auto.
+        ** right. inversion H0 as [t'' [a' He]]. exists t''. exists a'. subst. simpl. auto.
+  - intros. subst. induction es.
+Abort.
